Work from today, made theorem statement more complex as last one was provable just by executing/not interesting enough

prf/ELF_Relocation_Proof.thy
@@ -26,12 +26,13 @@ definition mov_constant_from_mem :: "64 word \<Rightarrow> instruction" where
 text {* The "fixed" program (i.e. the program that never changes and is never relocated) which
 moves the immediate constant 5 into a fixed address in memory and then moves that constant back into
 the RAX register using the two definitions above. *}
-definition fixed_program :: "8 word list" where
-  "fixed_program \<equiv>
-    List.concat (List.map encode [
-      mov_constant_to_mem (5 :: 64 word) (100 :: 64 word)
-    , mov_constant_from_mem (100 :: 64 word)
-    ])"
+definition fixed_program :: "nat \<Rightarrow> 8 word list" where
+  "fixed_program addr \<equiv>
+     let (addr::64 word) = of_nat addr in
+       List.concat (List.map encode [
+         mov_constant_to_mem (5 :: 64 word) addr
+      , mov_constant_from_mem addr
+      ])"
 
 text {* The program that will be relocated.  Moves an immediate constant 5 into some zero'd out
 address and will move the constant back again into the RAX register from the same address.  The zero'd
@@ -46,13 +47,14 @@ definition relocatable_program :: "8 word list" where
 text {* The relocation image that the linker produces internally after relocation.  The relocatable
 program above has now been relocated.  We will use this to populate a memory for the X64 emulation
 below. *}
-definition relocation_image :: "Abis.any_abi_feature annotated_memory_image" where
-  "relocation_image \<equiv> img1 relocatable_program"
+definition relocation_image :: "nat \<Rightarrow> Abis.any_abi_feature annotated_memory_image" where
+  "relocation_image addr \<equiv> img1 addr relocatable_program"
 
 text {* Produce an X64 memory (a map from addresses to bytes) out of a memory image that we will
 obtain from the relocation_image above. *}
 definition X64_memory_of_memory_image :: "memory_image \<Rightarrow> (nat \<Rightarrow> 8 word)" where
   "X64_memory_of_memory_image i addr =
+     (* XXX: must be a better way than this, surely... *)
      (let keys = Map.dom i in
       let rels = { s. \<forall>k \<in> keys. Some s = i k \<and> addr \<ge> the (startpos s) \<and> addr \<le> the (startpos s) + the (length1 s) } in
       let arb  = Set.the_elem rels in
@@ -72,22 +74,60 @@ definition load_relocated_program_image :: "memory_image \<Rightarrow> nat \<Rig
      , exception = NoException
      \<rparr>"
 
+text {* The following is a helper function that creates an association list of memory addresses and
+bytes which we will use to set up the initial memory (code) contents of the fixed program's initial
+X64 state. *}
+fun build_fixed_program_code_memory :: "8 word list \<Rightarrow> nat \<Rightarrow> (nat \<times> 8 word) list" where
+  "build_fixed_program_code_memory [] addr = []" |
+  "build_fixed_program_code_memory (x#xs) addr = (addr, x)#build_fixed_program_code_memory xs (Suc addr)"
+
+text {* Build the program memory for the fixed program. *}
+definition build_fixed_program_memory :: "nat \<Rightarrow> 8 word list \<Rightarrow> 64 word \<Rightarrow> 8 word" where
+  "build_fixed_program_memory entry_point program x \<equiv>
+     let code_mem = map_of (build_fixed_program_code_memory program entry_point) in
+       (case code_mem (unat x) of
+         None \<Rightarrow> 0
+       | Some x \<Rightarrow> x)"
+
 text {* Produces an initial state for the X64 emulation out of the encoded instructions of our fixed
 program above, and a fixed start address for the instruction pointer.  This start address must match
 the start address of the .text section specified in Test_image.thy. *}
 definition load_fixed_program_instructions :: "8 word list \<Rightarrow> nat \<Rightarrow> X64_state" where
   "load_fixed_program_instructions p entry_point \<equiv>
-     \<lparr> EFLAGS = Map.empty (* XXX: or False? *)
-     , MEM = \<lambda>x. p ! (unat x - entry_point)
-     , REG = \<lambda>x. (0 :: 64 word)
-     , RIP = of_nat entry_point
-     , exception = NoException
-     \<rparr>"
+       \<lparr> EFLAGS = Map.empty (* XXX: or False? *)
+       , MEM = build_fixed_program_memory entry_point p
+       , REG = \<lambda>x. (0 :: 64 word)
+       , RIP = of_nat entry_point
+       , exception = NoException
+       \<rparr>"
 
 text {* Executes two steps of the X64 emulation given a fixed X64 state, returning a new state.  This
 will be sufficient to execute both programs above to their conclusion. *}
 definition run_two_steps :: "X64_state \<Rightarrow> X64_state" where
   "run_two_steps \<sigma> \<equiv> snd (x64_next (snd (x64_next \<sigma>)))"
+
+definition address_is_disjoint_from_text_and_within_data_section :: "nat \<Rightarrow> nat \<Rightarrow> nat \<Rightarrow> nat \<Rightarrow> nat \<Rightarrow> bool" where
+  "address_is_disjoint_from_text_and_within_data_section addr text_start data_start program_len data_len \<equiv>
+     (* Address is not within data section *)
+     \<not> (addr \<ge> text_start \<and> addr \<le> text_start + program_len) \<and>
+       (addr \<ge> data_start \<and> addr \<le> data_start + data_len)"
+
+fun possible_addresses :: "nat \<Rightarrow> nat \<Rightarrow> nat \<Rightarrow> bool" where
+  "possible_addresses start 0 addr = (addr = start)" |
+  "possible_addresses start (Suc cnt) addr =
+     (addr = start \<or> possible_addresses (Suc start) cnt addr)"
+
+(* XXX: in library, somewhere?  find_theorems doesn't find it... *)
+lemma nat_lesseq_elim:
+  fixes m n :: nat
+  assumes "m \<le> n"
+  shows "m = n \<or> m < n"
+using assms by auto
+
+lemma possible_addresses_elim:
+  assumes "address_is_disjoint_from_text_and_within_data_section addr text_start data_start program_len data_len"
+  shows "possible_addresses data_start data_len addr"
+sorry
 
 text {* We now have our (rather silly) correctness property, which serves to demonstrate that our
 definitions are capable of supporting formal proof.  If we set the Isabelle execution mechanism up
@@ -97,37 +137,97 @@ steps and demonstrate that the contents of their registers are the same after ex
 particular, both RAX registers will contain the immediate constant, 5. *}
 definition correctness_property :: "bool" where
   "correctness_property \<equiv>
-     let entry  = 4194304 in
-     let fstate1 = load_fixed_program_instructions fixed_program entry in
-     let fstate2 = run_two_steps fstate1 in
-     let rstate1 = load_relocated_program_image (elements relocation_image) entry in
-     let rstate2 = run_two_steps rstate1 in
-       REG rstate2 = REG rstate2 \<and> (REG rstate1) RAX = 5"
+     \<forall>addr::nat.
+       let fprogr  = fixed_program addr in
+
+       let text_start   = 4194304 in (* Fixed in Test_image *)
+       let data_start   = 4194324 in (* Fixed in Test_image *)
+       let program_len  = List.length fprogr in
+       let data_len     = 8 in      (* Fixed in Test_image *)
+
+       let fstate1 = load_fixed_program_instructions fprogr text_start in
+       let fstate2 = run_two_steps fstate1 in
+       let rstate1 = load_relocated_program_image (elements (relocation_image addr)) text_start in
+       let rstate2 = run_two_steps rstate1 in
+
+       address_is_disjoint_from_text_and_within_data_section addr text_start data_start program_len data_len \<longrightarrow>
+           REG fstate2 = REG rstate2 \<and> (REG rstate1) RAX = 5"
 
 subsection {* Lemmas *}
 
-lemma encode_relocated_program_compute:
-  shows "map encode [
-           Zmov (Z_ALWAYS, Z64, Zrm_i (Zm (None, ZnoBase, 0), 5)),
-           Zmov (Z_ALWAYS, Z64, Zr_rm (RAX, Zm (None, ZnoBase, 0)))
-         ] = [[72, 199, 4, 37, 0, 0, 0, 0, 5, 0, 0, 0], [72, 139, 4, 37, 0, 0, 0, 0]]"
-sorry (* XXX: true by eval *)
+declare [[show_types]]
+
+(* XXX: ugly but necessary to control simplification below *)
+lemma possible_addresses_8_unfold:
+  fixes start addr :: nat
+  shows "possible_addresses start (8\<Colon>nat) addr = (addr = start \<or>
+         addr = Suc (start) \<or>
+         addr = Suc (Suc (start)) \<or>
+         addr = Suc (Suc (Suc (start))) \<or>
+         addr = Suc (Suc (Suc (Suc (start)))) \<or>
+         addr = Suc (Suc (Suc (Suc (Suc (start))))) \<or>
+         addr = Suc (Suc (Suc (Suc (Suc (Suc (start)))))) \<or>
+         addr = Suc (Suc (Suc (Suc (Suc (Suc (Suc (start))))))) \<or>
+         addr = Suc (Suc (Suc (Suc (Suc (Suc (Suc (Suc (start)))))))))"
+sorry
 
 lemma encode_fixed_program_compute:
-  shows "map encode [
-           Zmov (Z_ALWAYS, Z64, Zrm_i (Zm (None, ZnoBase, 100), 5)),
-           Zmov (Z_ALWAYS, Z64, Zr_rm (RAX, Zm (None, ZnoBase, 100)))
-         ] = [[72, 199, 4, 37, 100, 0, 0, 0, 5, 0, 0, 0], [72, 139, 4, 37, 100, 0, 0, 0]]"
-sorry (* XXX: true by eval *)
-
-lemma e_rm_imm_relocated_technical:
-  shows "List.concat [e_rm_imm (Z64, Zm (None, ZnoBase, 0), 5, 0, 198), e_rm_reg (Z64, Zm (None, ZnoBase, 0), word_of_int (int (Zreg_to_nat RAX)), [], 138)] =
-    [72, 199, 4, 37, 0, 0, 0, 0, 5, 0, 0, 0, 72, 139, 4, 37, 0, 0, 0, 0]"
-sorry (* XXX: true by eval *)
-
-lemma img1_technical:
-  shows "img1 [72, 199, 4, 37, 0, 0, 0, 0, 5, 0, 0, 0, 72, 139, 4, 37, 0, 0, 0, 0] = xxx"
-sorry
+  fixes addr :: nat
+  shows "possible_addresses 4194324 8 addr \<Longrightarrow>
+    let field = (20 + (addr - 4194324)) in
+    map encode [
+      Zmov (Z_ALWAYS, Z64, Zrm_i (Zm (None, ZnoBase, of_nat addr), 5))
+    , Zmov (Z_ALWAYS, Z64, Zr_rm (RAX, Zm (None, ZnoBase, of_nat addr)))
+    ] =
+    [[72\<Colon>8 word, 199\<Colon>8 word, 4\<Colon>8 word, 37\<Colon>8 word, of_nat field, 0\<Colon>8 word, 64\<Colon>8 word, 0\<Colon>8 word, 5\<Colon>8 word, 0\<Colon>8 word, 0\<Colon>8 word, 0\<Colon>8 word],
+     [72\<Colon>8 word, 139\<Colon>8 word, 4\<Colon>8 word, 37\<Colon>8 word, of_nat field, 0\<Colon>8 word, 64\<Colon>8 word, 0\<Colon>8 word]]"
+  apply(unfold possible_addresses_8_unfold)
+  apply(subgoal_tac "word_cat (0\<Colon>1 word) ((word_cat ((word_extract (3\<Colon>nat) (3\<Colon>nat) (0\<Colon>4 word))::1 word) (0\<Colon>2 word))::3 word) OR (8\<Colon>4 word) = (8::4 word)")
+  apply(erule disjE)
+    apply(simp only: list.map encode.simps Let_def)
+    apply(simp only: instruction.case split Zcond.case Zsize.case Zdest_src.case Zrm.case)
+    apply(simp only: Zreg_to_nat.simps Zreg.simps)
+    apply eval
+  apply(erule disjE)
+    apply(simp only: list.map encode.simps Let_def)
+    apply(simp only: instruction.case split Zcond.case Zsize.case Zdest_src.case Zrm.case)
+    apply(simp only: Zreg_to_nat.simps Zreg.simps)
+    apply eval
+  apply(erule disjE)
+    apply(simp only: list.map encode.simps Let_def)
+    apply(simp only: instruction.case split Zcond.case Zsize.case Zdest_src.case Zrm.case)
+    apply(simp only: Zreg_to_nat.simps Zreg.simps)
+    apply eval
+  apply(erule disjE)
+    apply(simp only: list.map encode.simps Let_def)
+    apply(simp only: instruction.case split Zcond.case Zsize.case Zdest_src.case Zrm.case)
+    apply(simp only: Zreg_to_nat.simps Zreg.simps)
+    apply eval
+  apply(erule disjE)
+    apply(simp only: list.map encode.simps Let_def)
+    apply(simp only: instruction.case split Zcond.case Zsize.case Zdest_src.case Zrm.case)
+    apply(simp only: Zreg_to_nat.simps Zreg.simps)
+    apply eval
+  apply(erule disjE)
+    apply(simp only: list.map encode.simps Let_def)
+    apply(simp only: instruction.case split Zcond.case Zsize.case Zdest_src.case Zrm.case)
+    apply(simp only: Zreg_to_nat.simps Zreg.simps)
+    apply eval
+  apply(erule disjE)
+    apply(simp only: list.map encode.simps Let_def)
+    apply(simp only: instruction.case split Zcond.case Zsize.case Zdest_src.case Zrm.case)
+    apply(simp only: Zreg_to_nat.simps Zreg.simps)
+    apply eval
+  apply(erule disjE)
+    apply(simp only: list.map encode.simps Let_def)
+    apply(simp only: instruction.case split Zcond.case Zsize.case Zdest_src.case Zrm.case)
+    apply(simp only: Zreg_to_nat.simps Zreg.simps)
+    apply eval
+    apply(simp only: list.map encode.simps Let_def)
+    apply(simp only: instruction.case split Zcond.case Zsize.case Zdest_src.case Zrm.case)
+    apply(simp only: Zreg_to_nat.simps Zreg.simps)
+    apply eval+
+done
 
 (* XXX: ugly, but necessary to control the simplifier below *)
 lemma for_loop_19_unroll:
@@ -148,402 +248,140 @@ lemma for_loop_19_unroll:
                                       (u, ua) \<Rightarrow> case act 6 ua of
                                                  (u, ua) \<Rightarrow> case act 5 ua of
                                                             (u, ua) \<Rightarrow> case act 4 ua of (u, ua) \<Rightarrow> case act 3 ua of (u, ua) \<Rightarrow> case act 2 ua of (u, ua) \<Rightarrow> case act 1 ua of (u, x) \<Rightarrow> act 0 x)"
-  by simp
+  apply simp
+done
 
-(* XXX: need some precondition on size of x, here, but that's fine as we only ever use this lemma on
-   small constants...
-*)
-lemma word_arith_technical:
-  shows "unat (of_nat 4194304 + word_of_int (int x)) = (4194304 + x)"
+lemma word_arith_technical1:
+  assumes "x < 2^64 - 4194304"
+  shows "(4194304\<Colon>64 word) + word_of_int (int (x\<Colon>nat)) = of_nat (4194304 + x)"
+sorry
+
+lemma word_arith_technical2:
+  assumes "x < 2^64 - 4194316"
+  shows "(4194316\<Colon>64 word) + word_of_int (int (x\<Colon>nat)) = of_nat (4194316 + x)"
 sorry
 
 lemma x64_fetch_fixed1:
-  shows "x64_fetch \<lparr>EFLAGS = Map.empty, MEM = \<lambda>x. [72, 199, 4, 37, 100, 0, 0, 0, 5, 0, 0, 0, 72, 139, 4, 37, 100, 0, 0, 0] ! (unat x - 4194304),
-                    REG = \<lambda>x. 0, RIP = of_nat 4194304, exception = NoException\<rparr> =
-          ([72, 199, 4, 37, 100, 0, 0, 0, 5, 0, 0, 0, 72, 139, 4, 37, 100, 0, 0, 0],
-           \<lparr>EFLAGS = Map.empty, MEM = \<lambda>x. [72, 199, 4, 37, 100, 0, 0, 0, 5, 0, 0, 0, 72, 139, 4, 37, 100, 0, 0, 0] ! (unat x - 4194304),
-            REG = \<lambda>x. 0, RIP = 4194304, exception = NoException\<rparr>)"
-apply(simp only: x64_fetch.simps for_loop_19_unroll)
-apply(simp only: snd_def split X64_state.simps fst_def)
-apply(simp only: word_arith_technical)
-apply simp
+  shows "x64_fetch \<lparr>EFLAGS = Map.empty,
+                              MEM = build_fixed_program_memory (4194304\<Colon>nat)
+                                     [72\<Colon>8 word, 199\<Colon>8 word, 4\<Colon>8 word, 37\<Colon>8 word, (20\<Colon>8 word) + of_nat (addr - (4194324\<Colon>nat)), 0\<Colon>8 word, 64\<Colon>8 word, 0\<Colon>8 word, 5\<Colon>8 word, 0\<Colon>8 word, 0\<Colon>8 word, 0\<Colon>8 word,
+                                      72\<Colon>8 word, 139\<Colon>8 word, 4\<Colon>8 word, 37\<Colon>8 word, (20\<Colon>8 word) + of_nat (addr - (4194324\<Colon>nat)), 0\<Colon>8 word, 64\<Colon>8 word, 0\<Colon>8 word],
+                              REG = \<lambda>x\<Colon>Zreg. 0\<Colon>64 word, RIP = 4194304\<Colon>64 word, exception = NoException\<rparr> =
+  ([72\<Colon>8 word, 199\<Colon>8 word, 4\<Colon>8 word, 37\<Colon>8 word, (20\<Colon>8 word) + of_nat (addr - (4194324\<Colon>nat)), 0\<Colon>8 word, 64\<Colon>8 word, 0\<Colon>8 word, 5\<Colon>8 word, 0\<Colon>8 word, 0\<Colon>8 word, 0\<Colon>8 word, 72\<Colon>8 word, 139\<Colon>8 word, 4\<Colon>8 word,
+      37\<Colon>8 word, (20\<Colon>8 word) + of_nat (addr - (4194324\<Colon>nat)), 0\<Colon>8 word, 64\<Colon>8 word, 0\<Colon>8 word],
+     \<lparr>EFLAGS = Map.empty,
+        MEM = build_fixed_program_memory (4194304\<Colon>nat)
+               [72\<Colon>8 word, 199\<Colon>8 word, 4\<Colon>8 word, 37\<Colon>8 word, (20\<Colon>8 word) + of_nat (addr - (4194324\<Colon>nat)), 0\<Colon>8 word, 64\<Colon>8 word, 0\<Colon>8 word, 5\<Colon>8 word, 0\<Colon>8 word, 0\<Colon>8 word, 0\<Colon>8 word, 72\<Colon>8 word, 139\<Colon>8 word,
+                4\<Colon>8 word, 37\<Colon>8 word, (20\<Colon>8 word) + of_nat (addr - (4194324\<Colon>nat)), 0\<Colon>8 word, 64\<Colon>8 word, 0\<Colon>8 word],
+        REG = \<lambda>x\<Colon>Zreg. 0\<Colon>64 word, RIP = 4194304\<Colon>64 word, exception = NoException\<rparr>)"
+  apply(simp only: x64_fetch.simps for_loop_19_unroll)
+  apply(simp only: split snd_def X64_state.simps fst_def)
+  apply(simp add: word_arith_technical1 build_fixed_program_memory_def)
 done
 
+value "x64_fetch \<lparr>EFLAGS = Map.empty,
+                              MEM = (build_fixed_program_memory (4194304\<Colon>nat)
+                                      [72\<Colon>8 word, 199\<Colon>8 word, 4\<Colon>8 word, 37\<Colon>8 word, (21\<Colon>8 word), 0\<Colon>8 word, 64\<Colon>8 word, 0\<Colon>8 word, 5\<Colon>8 word, 0\<Colon>8 word, 0\<Colon>8 word, 0\<Colon>8 word,
+                                       72\<Colon>8 word, 139\<Colon>8 word, 4\<Colon>8 word, 37\<Colon>8 word, (21\<Colon>8 word), 0\<Colon>8 word, 64\<Colon>8 word, 0\<Colon>8 word])
+                                (0::64 word := 5\<Colon>8 word, (1\<Colon>64 word) := 0\<Colon>8 word, (2\<Colon>64 word) := 0\<Colon>8 word, (3\<Colon>64 word) := 0\<Colon>8 word,
+                                 (4\<Colon>64 word) := 0\<Colon>8 word, (5\<Colon>64 word) := 0\<Colon>8 word, (6\<Colon>64 word) := 0\<Colon>8 word, (7\<Colon>64 word) := 0\<Colon>8 word),
+                              REG = \<lambda>x\<Colon>Zreg. 0\<Colon>64 word, RIP = 4194316\<Colon>64 word, exception = NoException\<rparr>"
+
+lemma x64_fetch_fixed2:
+  shows "x64_fetch \<lparr>EFLAGS = Map.empty,
+                              MEM = (build_fixed_program_memory (4194304\<Colon>nat)
+                                      [72\<Colon>8 word, 199\<Colon>8 word, 4\<Colon>8 word, 37\<Colon>8 word, (20\<Colon>8 word) + of_nat (addr - (4194324\<Colon>nat)), 0\<Colon>8 word, 64\<Colon>8 word, 0\<Colon>8 word, 5\<Colon>8 word, 0\<Colon>8 word, 0\<Colon>8 word, 0\<Colon>8 word,
+                                       72\<Colon>8 word, 139\<Colon>8 word, 4\<Colon>8 word, 37\<Colon>8 word, (20\<Colon>8 word) + of_nat (addr - (4194324\<Colon>nat)), 0\<Colon>8 word, 64\<Colon>8 word, 0\<Colon>8 word])
+                                (of_nat addr := 5\<Colon>8 word, of_nat addr + (1\<Colon>64 word) := 0\<Colon>8 word, of_nat addr + (2\<Colon>64 word) := 0\<Colon>8 word, (3\<Colon>64 word) + of_nat addr := 0\<Colon>8 word,
+                                 of_nat addr + (4\<Colon>64 word) := 0\<Colon>8 word, (5\<Colon>64 word) + of_nat addr := 0\<Colon>8 word, (6\<Colon>64 word) + of_nat addr := 0\<Colon>8 word, (7\<Colon>64 word) + of_nat addr := 0\<Colon>8 word),
+                              REG = \<lambda>x\<Colon>Zreg. 0\<Colon>64 word, RIP = 4194316\<Colon>64 word, exception = NoException\<rparr> =
+    ([72, 199, 4, 37, (20\<Colon>8 word) + of_nat (addr - (4194324\<Colon>nat)), 0, 64\<Colon>8 word, 0\<Colon>8 word, 5\<Colon>8 word, 0\<Colon>8 word, 0\<Colon>8 word, 0\<Colon>8 word, 72\<Colon>8 word, 139\<Colon>8 word, 4\<Colon>8 word,
+      37\<Colon>8 word, (20\<Colon>8 word) + of_nat (addr - (4194324\<Colon>nat)), 0\<Colon>8 word, 64\<Colon>8 word, 0\<Colon>8 word]@yy,
+     \<lparr>EFLAGS = Map.empty, MEM = (build_fixed_program_memory (4194304\<Colon>nat)
+                                      [72\<Colon>8 word, 199\<Colon>8 word, 4\<Colon>8 word, 37\<Colon>8 word, (21\<Colon>8 word), 0\<Colon>8 word, 64\<Colon>8 word, 0\<Colon>8 word, 5\<Colon>8 word, 0\<Colon>8 word, 0\<Colon>8 word, 0\<Colon>8 word,
+                                       72\<Colon>8 word, 139\<Colon>8 word, 4\<Colon>8 word, 37\<Colon>8 word, (21\<Colon>8 word), 0\<Colon>8 word, 64\<Colon>8 word, 0\<Colon>8 word])
+                                (0::64 word := 5\<Colon>8 word, (1\<Colon>64 word) := 0\<Colon>8 word, (2\<Colon>64 word) := 0\<Colon>8 word, (3\<Colon>64 word) := 0\<Colon>8 word,
+                                 (4\<Colon>64 word) := 0\<Colon>8 word, (5\<Colon>64 word) := 0\<Colon>8 word, (6\<Colon>64 word) := 0\<Colon>8 word, (7\<Colon>64 word) := 0\<Colon>8 word),
+                              REG = \<lambda>x\<Colon>Zreg. 0\<Colon>64 word, RIP = 4194316\<Colon>64 word, exception = NoException\<rparr>)"
+  apply(simp only: x64_fetch.simps for_loop_19_unroll)
+  apply(simp only: split snd_def fst_def X64_state.simps)
+  apply(simp add: word_arith_technical2 build_fixed_program_memory_def)
+
 lemma x64_decode_fixed1:
-  shows "x64_decode [72, 199, 4, 37, 100, 0, 0, 0, 5, 0, 0, 0, 72, 139, 4, 37, 100, 0, 0, 0] =
-    Zfull_inst ([], Zmov (Z_ALWAYS, Z64, Zrm_i (Zm (None, ZnoBase, 100), 5)), [72, 139, 4, 37, 100, 0, 0, 0])"
-sorry (* XXX: true by eval *)
-
-lemma finite_maps_equal:
-  fixes f1 f2 :: "'a \<rightharpoonup> 'b"
-  assumes "\<forall>x \<in> dom f1 \<union> dom f2. f1 x = f2 x"
-  shows "f1 = f2"
+  fixes addr :: nat
+  shows "x64_decode
+           [72\<Colon>8 word, 199\<Colon>8 word, 4\<Colon>8 word, 37\<Colon>8 word, (20\<Colon>8 word) + of_nat (addr - (4194324\<Colon>nat)), 0\<Colon>8 word, 64\<Colon>8 word, 0\<Colon>8 word, 5\<Colon>8 word, 0\<Colon>8 word, 0\<Colon>8 word, 0\<Colon>8 word, 72\<Colon>8 word, 139\<Colon>8 word,
+            4\<Colon>8 word, 37\<Colon>8 word, (20\<Colon>8 word) + of_nat (addr - (4194324\<Colon>nat)), 0\<Colon>8 word, 64\<Colon>8 word, 0\<Colon>8 word] =
+         Zfull_inst ([], Zmov (Z_ALWAYS, Z64, Zrm_i (Zm (None, ZnoBase, of_nat addr\<Colon>64 word), 5\<Colon>64 word)), [72\<Colon>8 word, 139\<Colon>8 word, 4\<Colon>8 word, 37\<Colon>8 word, (20\<Colon>8 word) + of_nat (addr - (4194324\<Colon>nat)), 0\<Colon>8 word, 64\<Colon>8 word, 0\<Colon>8 word])"
 sorry
-
-declare [[show_types]]
-
-lemma Run_technical_fixed1:
-  shows "Run (Zmov (Z_ALWAYS, Z64, Zrm_i (Zm (None, ZnoBase, 100), 5)))
-     \<lparr>EFLAGS = Map.empty, MEM = \<lambda>x. [72, 199, 4, 37, 100, 0, 0, 0, 5, 0, 0, 0, 72, 139, 4, 37, 100, 0, 0, 0] ! (unat x - 4194304), REG = \<lambda>x. 0,
-        RIP = of_nat 4194304 + word_of_int (int (20 - length [72::8 word, 139, 4, 37, 100, 0, 0, 0])), exception = NoException\<rparr> =
-     ((), \<lparr>EFLAGS = Map.empty,
-            MEM = (\<lambda>x. [72, 199, 4, 37, 100, 0, 0, 0, 5, 0, 0, 0, 72, 139, 4, 37, 100, 0, 0, 0] ! (unat x - 4194304))
-              (100 := word_extract 7 0 (word_extract 15 0 (word_extract 31 0 (5::64 word))), 101 := word_extract 15 8 (word_extract 15 0 (word_extract 31 0 (5::64 word))),
-               102 := word_extract 7 0 (word_extract 31 16 (word_extract 31 0 (5::64 word))), 103 := word_extract 15 8 (word_extract 31 16 (word_extract 31 0 (5::64 word))),
-               104 := word_extract 7 0 (word_extract 15 0 (word_extract 63 32 (5::64 word))), 105 := word_extract 15 8 (word_extract 15 0 (word_extract 63 32 (5::64 word))),
-               106 := word_extract 7 0 (word_extract 31 16 (word_extract 63 32 (5::64 word))), 107 := word_extract 15 8 (word_extract 31 16 (word_extract 63 32 (5::64 word)))),
-            REG = \<lambda>x. 0, RIP = (of_nat 4194316)::64 word, exception = NoException\<rparr>)"
-  apply(simp only: Run.simps instruction.case dfn'Zmov.simps read_cond.simps Zcond.simps)
-  apply(simp only: Let_def split if_True fst_def EA.simps ea_Zsrc.simps Zdest_src.case)
-  apply(simp only: Zea.case restrictSize.simps Zsize.case split ea_Zdest.simps)
-  apply(simp only: Zdest_src.case split write'EA.simps fst_def ea_Zrm.simps Zrm.case ea_index.simps)
-  apply(simp only: option.case split Zea.case Zsize.case ea_base.simps Zbase.simps)
-  apply(simp only: write'mem64.simps write'mem32.simps write'mem16.simps write'mem8.simps)
-  apply(simp only: snd_def split X64_state.simps Pair_eq)
-  apply(rule conjI, simp only: refl; simp only: X64_state.ext_inject)
-  apply(simp only: refl simp_thms)
-  apply(rule conjI)
-  sorry (* XXX: weird problem with types, here *)
-
-declare [[show_types]]
 
 lemma x64_next_fixed1:
   shows "x64_next \<lparr>EFLAGS = Map.empty,
-                                          MEM = \<lambda>x\<Colon>64 word. [72\<Colon>8 word, 199\<Colon>8 word, 4\<Colon>8 word, 37\<Colon>8 word, 100\<Colon>8 word, 0\<Colon>8 word, 0\<Colon>8 word, 0\<Colon>8 word, 5\<Colon>8 word, 0\<Colon>8 word, 0\<Colon>8 word, 0\<Colon>8 word, 72\<Colon>8 word,
-                                                             139\<Colon>8 word, 4\<Colon>8 word, 37\<Colon>8 word, 100\<Colon>8 word, 0\<Colon>8 word, 0\<Colon>8 word, 0\<Colon>8 word] !
-                                                            (unat x - (4194304\<Colon>nat)),
-                                          REG = \<lambda>x\<Colon>Zreg. 0\<Colon>64 word, RIP = of_nat (4194304\<Colon>nat), exception = NoException\<rparr> =
-         ((), \<lparr>EFLAGS = Map.empty,
-            MEM = (\<lambda>x. [72, 199, 4, 37, 100, 0, 0, 0, 5, 0, 0, 0, 72, 139, 4, 37, 100, 0, 0, 0] ! (unat x - 4194304))
-              (100 := word_extract 7 0 (word_extract 15 0 (word_extract 31 0 (5::64 word))), 101 := word_extract 15 8 (word_extract 15 0 (word_extract 31 0 (5::64 word))),
-               102 := word_extract 7 0 (word_extract 31 16 (word_extract 31 0 (5::64 word))), 103 := word_extract 15 8 (word_extract 31 16 (word_extract 31 0 (5::64 word))),
-               104 := word_extract 7 0 (word_extract 15 0 (word_extract 63 32 (5::64 word))), 105 := word_extract 15 8 (word_extract 15 0 (word_extract 63 32 (5::64 word))),
-               106 := word_extract 7 0 (word_extract 31 16 (word_extract 63 32 (5::64 word))), 107 := word_extract 15 8 (word_extract 31 16 (word_extract 63 32 (5::64 word)))),
-            REG = \<lambda>x. 0, RIP = of_nat 4194316, exception = NoException\<rparr>)"
-  apply(simp only: x64_next.simps x64_fetch_fixed1 fst_def split)
-  apply(simp only: x64_decode_fixed1 Zinst.case split X64_state.simps Run_technical_fixed1 word_arith_technical)
-done
+                                     MEM = build_fixed_program_memory (4194304\<Colon>nat)
+                                            [72\<Colon>8 word, 199\<Colon>8 word, 4\<Colon>8 word, 37\<Colon>8 word, (20\<Colon>8 word) + of_nat (addr - (4194324\<Colon>nat)), 0\<Colon>8 word, 64\<Colon>8 word, 0\<Colon>8 word, 5\<Colon>8 word, 0\<Colon>8 word, 0\<Colon>8 word,
+                                             0\<Colon>8 word, 72\<Colon>8 word, 139\<Colon>8 word, 4\<Colon>8 word, 37\<Colon>8 word, (20\<Colon>8 word) + of_nat (addr - (4194324\<Colon>nat)), 0\<Colon>8 word, 64\<Colon>8 word, 0\<Colon>8 word],
+                                     REG = \<lambda>x\<Colon>Zreg. 0\<Colon>64 word, RIP = 4194304\<Colon>64 word, exception = NoException\<rparr> = ((), \<lparr>EFLAGS = Map.empty,
+            MEM = (build_fixed_program_memory (4194304\<Colon>nat)
+                    [72\<Colon>8 word, 199\<Colon>8 word, 4\<Colon>8 word, 37\<Colon>8 word, (20\<Colon>8 word) + of_nat (addr - (4194324\<Colon>nat)), 0\<Colon>8 word, 64\<Colon>8 word, 0\<Colon>8 word, 5\<Colon>8 word, 0\<Colon>8 word, 0\<Colon>8 word, 0\<Colon>8 word, 72\<Colon>8 word,
+                     139\<Colon>8 word, 4\<Colon>8 word, 37\<Colon>8 word, (20\<Colon>8 word) + of_nat (addr - (4194324\<Colon>nat)), 0\<Colon>8 word, 64\<Colon>8 word, 0\<Colon>8 word])
+              (of_nat addr := 5::8 word,
+               of_nat addr + (1\<Colon>64 word) := 0::8 word,
+               of_nat addr + (2\<Colon>64 word) := 0::8 word,
+               (3\<Colon>64 word) + of_nat addr := 0::8 word, of_nat addr + (4\<Colon>64 word) := 0\<Colon>8 word,
+               (5\<Colon>64 word) + of_nat addr := 0\<Colon>8 word, (6\<Colon>64 word) + of_nat addr := 0\<Colon>8 word, (7\<Colon>64 word) + of_nat addr := 0\<Colon>8 word),
+            REG = \<lambda>x\<Colon>Zreg. 0\<Colon>64 word, RIP = 4194316\<Colon>64 word, exception = NoException\<rparr>)"
+  apply(simp only: x64_next.simps)
+  apply(simp only: x64_fetch_fixed1 fst_def split)
+  apply(simp only: x64_decode_fixed1)
+  apply(simp only: Zinst.case split X64_state.simps)
+  apply simp (* XXX: true by eval *)
+sorry
+
+lemma x64_next_fixed2:
+  shows "x64_next \<lparr>EFLAGS = Map.empty,
+                      MEM = (build_fixed_program_memory (4194304\<Colon>nat)
+                              [72\<Colon>8 word, 199\<Colon>8 word, 4\<Colon>8 word, 37\<Colon>8 word, (20\<Colon>8 word) + of_nat (addr - (4194324\<Colon>nat)), 0\<Colon>8 word, 64\<Colon>8 word, 0\<Colon>8 word, 5\<Colon>8 word, 0\<Colon>8 word, 0\<Colon>8 word, 0\<Colon>8 word,
+                               72\<Colon>8 word, 139\<Colon>8 word, 4\<Colon>8 word, 37\<Colon>8 word, (20\<Colon>8 word) + of_nat (addr - (4194324\<Colon>nat)), 0\<Colon>8 word, 64\<Colon>8 word, 0\<Colon>8 word])
+                        (of_nat addr := 5\<Colon>8 word, of_nat addr + (1\<Colon>64 word) := 0\<Colon>8 word, of_nat addr + (2\<Colon>64 word) := 0\<Colon>8 word, (3\<Colon>64 word) + of_nat addr := 0\<Colon>8 word,
+                         of_nat addr + (4\<Colon>64 word) := 0\<Colon>8 word, (5\<Colon>64 word) + of_nat addr := 0\<Colon>8 word, (6\<Colon>64 word) + of_nat addr := 0\<Colon>8 word, (7\<Colon>64 word) + of_nat addr := 0\<Colon>8 word),
+                      REG = \<lambda>x\<Colon>Zreg. 0\<Colon>64 word, RIP = 4194316\<Colon>64 word, exception = NoException\<rparr> = xxx"
+  apply(simp only: x64_next.simps)
+
+lemma run_two_steps_fixed:
+  shows "(run_two_steps
+                      \<lparr>EFLAGS = Map.empty,
+                         MEM = build_fixed_program_memory (4194304\<Colon>nat)
+                                [72\<Colon>8 word, 199\<Colon>8 word, 4\<Colon>8 word, 37\<Colon>8 word, (20\<Colon>8 word) + of_nat (addr - (4194324\<Colon>nat)), 0\<Colon>8 word, 64\<Colon>8 word, 0\<Colon>8 word, 5\<Colon>8 word, 0\<Colon>8 word, 0\<Colon>8 word, 0\<Colon>8 word,
+                                 72\<Colon>8 word, 139\<Colon>8 word, 4\<Colon>8 word, 37\<Colon>8 word, (20\<Colon>8 word) + of_nat (addr - (4194324\<Colon>nat)), 0\<Colon>8 word, 64\<Colon>8 word, 0\<Colon>8 word],
+                         REG = \<lambda>x\<Colon>Zreg. 0\<Colon>64 word, RIP = 4194304\<Colon>64 word, exception = NoException\<rparr>) = xxx"
+  apply(simp only: run_two_steps_def snd_def)
+  apply(simp only: x64_next_fixed1 split)
 
 subsection {* The "big" theorem *}
 
 text {* Finally, our correctness theorem which shows that our correctness property holds: *}
 theorem correctness_property_True:
   shows "correctness_property"
-unfolding correctness_property_def
-  (* Get rid of the entry address... *)
-  apply(subst Let_def)
-  (* Start working on the fixed program, first: *)
-  apply(simp only: fixed_program_def mov_constant_to_mem_def mov_constant_from_mem_def)
-  apply(simp only: encode_fixed_program_compute concat.simps append.simps)
-  apply(simp only: load_fixed_program_instructions_def)
-  (* Start running the two steps of the fixed program: *)
-  apply(subst Let_def)
-  apply(simp only: run_two_steps_def)
-(*
-  (* Start working on the relocated program, now: *)
-  apply(simp only: relocation_image_def relocatable_program_def mov_constant_to_mem_def mov_constant_from_mem_def)
-  apply(simp only: list.map encode.simps encode_relocated_program_compute)
-  apply(simp only: instruction.case split Zcond.case Zsize.case Zdest_src.case Zrm.case)
-  apply(simp only: e_rm_imm_relocated_technical)
-*)
-
-term Zm
-
-(*
-section {* OLD STUFF *}
-
-definition mov_constant_to_mem :: "64 word \<Rightarrow> 64 word \<Rightarrow> instruction" where
-  "mov_constant_to_mem constant addr \<equiv> Zmov (Z_ALWAYS, (Z64, Zrm_i (Zm (None, (ZnoBase, addr)), constant)))"
-
-definition mov_constant_from_mem :: "64 word \<Rightarrow> instruction" where
-  "mov_constant_from_mem addr \<equiv> Zmov (Z_ALWAYS, (Z64, Zr_rm (RAX, Zm (None, (ZnoBase, addr)))))"
-
-definition fixed_program :: "8 word list" where
-  "fixed_program \<equiv>
-    List.concat (List.map encode [
-      mov_constant_to_mem (5 :: 64 word) (100 :: 64 word)
-    , mov_constant_from_mem (100 :: 64 word)
-    ])"
-
-definition relocatable_program :: "8 word list" where
-  "relocatable_program \<equiv>
-     List.concat (List.map encode [
-       mov_constant_to_mem (5 :: 64 word) (0 :: 64 word)
-     , mov_constant_from_mem (0 :: 64 word)
-     ])"
-
-definition relocation_image :: "Abis.any_abi_feature annotated_memory_image" where
-  "relocation_image \<equiv> img1 relocatable_program"
-
-fun X64_memory_of_memory_image :: "memory_image \<Rightarrow> (nat \<Rightarrow> 8 word)" where
-  "X64_memory_of_memory_image i addr =
-     (let keys = Map.dom i in
-      let rels = { s. \<forall>k \<in> keys. Some s = i k \<and> addr \<ge> the (startpos s) \<and> addr \<le> the (startpos s) + the (length1 s) } in
-      let arb  = Set.the_elem rels in
-      let reba = addr - the (startpos arb) in
-      let byte = List.nth (contents arb) reba in
-        the byte)"
-
-definition load_image :: "memory_image \<Rightarrow> nat \<Rightarrow> X64_state" where
-  "load_image i entry_point \<equiv>
-     \<lparr> EFLAGS = \<lambda>x. None (* XXX: or False? *)
-     , MEM = \<lambda>a. X64_memory_of_memory_image i (unat a)
-     , REG = \<lambda>x. (0 :: 64 word)
-     , RIP = of_nat entry_point
-     , exception = NoException
-     \<rparr>"
-
-definition load_program :: "8 word list \<Rightarrow> nat \<Rightarrow> X64_state" where
-  "load_program p entry_point \<equiv>
-     \<lparr> EFLAGS = Map.empty (* XXX: or False? *)
-     , MEM = \<lambda>x. p ! (unat x - entry_point)
-     , REG = \<lambda>x. (0 :: 64 word)
-     , RIP = of_nat entry_point
-     , exception = NoException
-     \<rparr>"
-
-definition execute_two_steps :: "X64_state \<Rightarrow> X64_state" where
-  "execute_two_steps \<sigma> =
-     (let (fetched, \<sigma>') = x64_fetch \<sigma> in
-      let decoded = x64_decode fetched in
-       (case decoded of
-         Zfull_inst (pre, instr, suf) \<Rightarrow>
-           (let (_, \<sigma>'') = Run instr \<sigma>' in
-            let (fetched, \<sigma>''') = x64_fetch \<sigma>'' in
-            let decoded = x64_decode fetched in
-              (case decoded of
-                Zfull_inst (pre, instr, suf) \<Rightarrow>
-                let (_, \<sigma>'''') = Run instr \<sigma>''' in
-                  \<sigma>''''
-              | _ \<Rightarrow> undefined))
-       | _ \<Rightarrow> undefined))"
-
-lemma let_ext:
-  shows "let (x, y) = (u, v) in q x y = q u v"
-by auto
-
-lemma swap_pairs_lemma:
-  shows "swap_pairs {(Some (''.text'', 1, 4), SymbolRef ref_and_reloc_rec0), (Some (''.data'', 0, 8), SymbolDef def_rec0)} =
-      {(SymbolRef ref_and_reloc_rec0, Some (''.text'', 1, 4)), (SymbolDef def_rec0, Some (''.data'', 0, 8))}"
-  apply(simp add: swap_pairs_def)
-  apply auto
-done
-
-
-(* XXX: ugly, but necessary to control the simplifier below *)
-lemma for_loop_19_unroll:
-  fixes act :: "nat \<Rightarrow> 'a \<Rightarrow> (unit \<times> 'a)"
-  shows "for_loop ((19::nat), 0, act) = (\<lambda>u. case act 19 u of
-     (u, ua) \<Rightarrow> case act 18 ua of
-                (u, ua) \<Rightarrow> case act 17 ua of
-                           (u, ua) \<Rightarrow> case act 16 ua of
-                                      (u, ua) \<Rightarrow> case act 15 ua of
-                                                 (u, ua) \<Rightarrow> case act 14 ua of
-                                                            (u, ua) \<Rightarrow> case act 13 ua of
-                                                                       (u, ua) \<Rightarrow> case act 12 ua of
-                                                                                  (u, ua) \<Rightarrow> case act 11 ua of
-                                                                                             (u, ua) \<Rightarrow> case act 10 ua of
-     (u, ua) \<Rightarrow> case act 9 ua of
-                (u, ua) \<Rightarrow> case act 8 ua of
-                           (u, ua) \<Rightarrow> case act 7 ua of
-                                      (u, ua) \<Rightarrow> case act 6 ua of
-                                                 (u, ua) \<Rightarrow> case act 5 ua of
-                                                            (u, ua) \<Rightarrow> case act 4 ua of (u, ua) \<Rightarrow> case act 3 ua of (u, ua) \<Rightarrow> case act 2 ua of (u, ua) \<Rightarrow> case act 1 ua of (u, x) \<Rightarrow> act 0 x)"
-  by simp
- 
-lemma dom_lemma:
-  shows "{a. [''.text'' \<mapsto>
-                      \<lparr>startpos = Some 4194304, length1 = Some 20,
-                         contents = map Some (e_rm_imm (Z64, Zm (None, ZnoBase, 0), 5, 0, 198)) @ map Some (e_rm_reg (Z64, Zm (None, ZnoBase, 0), word_of_int (int (Zreg_to_nat RAX)), [], 138))\<rparr>,
-                      ''.data'' \<mapsto> \<lparr>startpos = Some 4194324, length1 = Some 8, contents = map Some (replicate 8 (of_nat 42))\<rparr>]
-                      a \<noteq>
-                     None} = { ''.text'', ''.data''}"
-  by auto
-
-lemma rels_lemma:
-  shows "{s. \<forall>k\<in>{''.text'', ''.data''}.
-                        Some s = [''.text'' \<mapsto>
-                                  \<lparr>startpos = Some 4194304, length1 = Some 20,
-                                     contents = map Some (e_rm_imm (Z64, Zm (None, ZnoBase, 0), 5, 0, 198)) @
-                                                map Some (e_rm_reg (Z64, Zm (None, ZnoBase, 0), word_of_int (int (Zreg_to_nat RAX)), [], 138))\<rparr>,
-                                  ''.data'' \<mapsto> \<lparr>startpos = Some 4194324, length1 = Some 8, contents = map Some (replicate 8 (of_nat 42))\<rparr>]
-                                  k \<and>
-                        the (startpos s) \<le> off \<and> off \<le> the (startpos s) + the (length1 s)} =
-                               { \<lparr>startpos = Some 4194304, length1 = Some 16,
-                                            contents = map Some (e_rm_imm (Z64, Zm (None, ZnoBase, 0), 5, 0, 198)) @
-                                                       map Some (e_rm_reg (Z64, Zm (None, ZnoBase, 0), word_of_int (int (Zreg_to_nat RAX)), [], 138))\<rparr> }"
-sorry
-
-lemma the_elem_lemma:
-  shows "the_elem { e } = e"
-  by auto
-
-lemma word_calc_lemma:
-  shows "unat (of_nat 4194304 + word_of_int (int x)) = 4194304 + x"
-sorry
-
-lemma the_startpos_lemma:
-  shows "the (startpos \<lparr>startpos = Some 4194304, length1 = Some 20,
-                                  contents = map Some (e_rm_imm (Z64, Zm (None, ZnoBase, 0), 5, 0, 198)) @
-                                             map Some (e_rm_reg (Z64, Zm (None, ZnoBase, 0), word_of_int (int (Zreg_to_nat RAX)), [], 138))\<rparr>) = 4194304"
-  by auto
-
-lemma signed_arith_lemma1:
-  shows "(18446744071562067968 <=s 0 \<and> 0 <=s 2147483647) = True"
-sorry
-
-lemma signed_arith_lemma2:
-  shows "(18446744071562067968 <=s 5 \<and> 5 <=s 2147483647) = True"
-sorry
-
-lemma signed_arith_lemma3:
-  shows "(18446744071562067968 <=s 100 \<and> 100 <=s 2147483647) = True"
-sorry
-
-value "((word_cat (0::32 word) (word_cat ((word_extract 3 3 0)::16 word) (0::16 word)))::64 word) OR (8::64 word)"
-
-lemma word_cat_lemma:
-  shows "(word_cat 0 (word_cat (word_extract 3 3 0) 0) OR 8 = 0) = True"
-sorry
-
-lemma x64_fetch_lemma1:
-  shows "x64_fetch \<lparr>EFLAGS = Map.empty,
-                        MEM = \<lambda>a. X64_memory_of_memory_image
-                                   [''.text'' \<mapsto>
-                                    \<lparr>startpos = Some 4194304, length1 = Some 20,
-                                       contents = map Some (e_rm_imm (Z64, Zm (None, ZnoBase, 0), 5, 0, 198)) @
-                                                  map Some (e_rm_reg (Z64, Zm (None, ZnoBase, 0), word_of_int (int (Zreg_to_nat RAX)), [], 138))\<rparr>,
-                                    ''.data'' \<mapsto> \<lparr>startpos = Some 4194324, length1 = Some 8, contents = map Some (replicate 8 (of_nat 42))\<rparr>]
-                                   (unat a),
-                        REG = \<lambda>x. 0, RIP = of_nat 4194304, exception = NoException\<rparr> = ([72, 199, 4, 37, 0, 0, 0, 0, 5, 0, 0, 0], \<lparr>EFLAGS = Map.empty, MEM = \<lambda>a. the ([] ! (unat a - 4194304)), REG = \<lambda>x. 0, RIP = 4194316, exception = NoException\<rparr>)"
-sorry
-
-lemma x64_fetch_lemma2:
-  shows "x64_fetch (load_program fixed_program 4194304) = ([72, 199, 4, 37, 0, 0, 0, 0, 5, 0, 0, 0], \<lparr>EFLAGS = Map.empty, MEM = \<lambda>a. the ([] ! (unat a - 4194304)), REG = \<lambda>x. 0, RIP = 4194316, exception = NoException\<rparr>)"
-sorry
-
-value "x64_decode
-               (fst (snd (for_loop (19, 0, \<lambda>i state. ((), MEM (snd state) (RIP (snd state) + word_of_int (int i)) # fst state, snd state))
-                           ([], \<lparr>EFLAGS = Map.empty, MEM = \<lambda>x. fixed_program ! (unat x - 4194304), REG = \<lambda>x. 0, RIP = of_nat 4194304, exception = NoException\<rparr>))))"
-
-lemma x64_decode_lemma1:
-  shows "x64_decode
-               (fst (snd (for_loop (19, 0, \<lambda>i state. ((), MEM (snd state) (RIP (snd state) + word_of_int (int i)) # fst state, snd state))
-                           ([], \<lparr>EFLAGS = Map.empty, MEM = \<lambda>x. fixed_program ! (unat x - 4194304), REG = \<lambda>x. 0, RIP = of_nat 4194304, exception = NoException\<rparr>)))) = xxx"
-
-(*  apply(simp only: x64_fetch.simps)
-  apply(simp only: Let_def)
-  apply(simp only: for_loop_19_unroll)
-  apply(simp only: split fst_def snd_def)
-  apply(simp only: X64_state.simps)
-  apply(simp only: X64_memory_of_memory_image.simps)
-
-  apply(simp only: dom_def; simp only: dom_lemma)
-
-  apply(subst Let_def; simp only: let_weak_cong[OF rels_lemma];
-          subst Let_def; simp only: the_elem_lemma; subst Let_def; simp only: element.simps option.sel word_calc_lemma;
-          subst Let_def; subst Let_def)+
-  apply(simp only: e_rm_reg.simps e_rm_imm.simps)
-  apply(simp only: e_ModRM.simps Zrm.case split option.case Zbase.case)
-  apply(simp only: e_imm32.simps)
-  apply(simp only: signed_arith_lemma1 if_True list.case split append.simps)
-  apply(simp only: e_opsize_imm.simps e_opsize.simps Zsize.case Let_def split)
-  apply(simp only: refl simp_thms if_True Zsize.case)
-  apply(simp only: e_imm32.simps signed_arith_lemma2 if_True list.case option.case split)
-  apply(simp only: concat.simps append.simps)
-  apply(simp only: rex_prefix.simps word_cat_lemma if_True append.simps list.map nth.simps)
-  apply simp
-(*
-  list.case split list.map append.simps)
-  apply(simp only: e_gen_rm_reg.simps)
-  apply(simp only: e_ModRM.simps Zrm.case split option.case Zbase.case)
-  apply(simp only: e_imm32.simps; simp only: signed_arith_lemma if_False list.case split list.map append.simps)
-  apply(simp)
-*)
-oops
-*)
-
-(*
-  apply(subst Let_def; simp only: let_weak_cong[OF rels_lemma];
-          subst Let_def; simp only: the_elem_lemma; subst Let_def; simp only: element.simps option.sel word_calc_lemma;
-          subst Let_def; subst Let_def)
-*)
-(*
-  apply(simp only: dom_def)
-  apply(simp only: dom_lemma)
-  apply(subst Let_def)
-  apply(simp only: let_weak_cong[OF rels_lemma])
-  apply(subst Let_def)
-  apply(simp only: the_elem_lemma)
-  apply(subst Let_def)
-  apply(simp only: word_calc_lemma)
-  apply(simp only: the_startpos_lemma)
-  apply(subst Let_def)
-  apply(simp only: element.simps)
-  apply(subst diff_self_eq_0)
-  apply(subst Let_def)
-*)
-
-lemma x64_decode_lemma:
-  shows "x64_decode [72, 199, 4, 37, 0, 0, 0, 0, 5, 0, 0, 0] = Zfull_inst ([], Zmov (Z_ALWAYS, Z64, Zrm_i (Zm (None, ZnoBase, 0), 5)), [])"
-by eval
-
-lemma subst_hyp:
-  assumes "x = y" and "P x \<Longrightarrow> Q"
-  shows "P y \<Longrightarrow> Q"
-using assms by auto
-
-theorem at_least_some_relocations_relocate:
-    fixes ef :: elf64_file and segs_and_provenance :: "(elf64_interpreted_segment \<times> segment_provenance) list" and entry :: "nat"
-            and rstate final_fixed_state final_relocatable_state :: "X64_state"
-  assumes "i = elements relocation_image" and "entry = 4194304"
-      and "rstate = load_image i entry"
-      and "fstate = load_program fixed_program entry"
-      and "final_fixed_state = execute_two_steps fstate"
-      and "final_relocatable_state = execute_two_steps rstate"
-    shows "REG final_fixed_state = REG final_relocatable_state" (* XXX: probably want to say something about the contents of memory here, too! *)
-using assms
-  apply(simp only: relocation_image_def)
-  apply(simp only: relocatable_program_def)
-  apply(simp only: List.list.map)
+  (* Unfold the lemma statement *)
+  apply(simp only: correctness_property_def)
+  apply(rule allI)
+  (* Start work on the fixed program *)
+  apply(simp only: fixed_program_def)
   apply(simp only: mov_constant_to_mem_def mov_constant_from_mem_def)
-  apply(simp only: encode.simps)
-  apply(simp only: X64.instruction.case split X64.Zcond.case Zsize.case Zdest_src.case Zrm.case)
-  apply(simp only: List.concat.simps)
-  apply(simp only: img1_def)
-  apply(simp only: rev.simps append.simps map_of.simps fst_def snd_def split)
-  apply(simp only: Let_def append_Nil2)
-  apply(simp only: meta0_def set_simps by_tag_from_by_range_def swap_pairs_lemma)
-  apply(simp only: map_append)
-  apply(simp only: relocate_output_image_def)
-  apply(simp only: annotated_memory_image.simps)
-  apply(simp only: lookupBy0_def)
-  apply(case_tac "findLowestKVWithKEquivTo (instance_Basic_classes_Ord_Memory_image_range_tag_dict instance_Basic_classes_Ord_Abis_any_abi_feature_dict)
-                          (instance_Basic_classes_Ord_Maybe_maybe_dict
-                            (instance_Basic_classes_Ord_tup2_dict instance_Basic_classes_Ord_string_dict
-                              (instance_Basic_classes_Ord_tup2_dict instance_Basic_classes_Ord_Num_natural_dict instance_Basic_classes_Ord_Num_natural_dict)))
-                          (SymbolRef null_symbol_reference_and_reloc_site) (tagEquiv instance_Abi_classes_AbiFeatureTagEquiv_Abis_any_abi_feature_dict)
-                          {(SymbolRef ref_and_reloc_rec0, Some (''.text'', 1\<Colon>nat, 4\<Colon>nat)), (SymbolDef def_rec0, Some (''.data'', 0\<Colon>nat, 8\<Colon>nat))} None")
   apply(simp only: Let_def)
-  apply(erule subst_hyp[where y ="None" and x="findLowestKVWithKEquivTo (instance_Basic_classes_Ord_Memory_image_range_tag_dict instance_Basic_classes_Ord_Abis_any_abi_feature_dict)
-                          (instance_Basic_classes_Ord_Maybe_maybe_dict
-                            (instance_Basic_classes_Ord_tup2_dict instance_Basic_classes_Ord_string_dict
-                              (instance_Basic_classes_Ord_tup2_dict instance_Basic_classes_Ord_Num_natural_dict instance_Basic_classes_Ord_Num_natural_dict)))
-                          (SymbolRef null_symbol_reference_and_reloc_site) (tagEquiv instance_Abi_classes_AbiFeatureTagEquiv_Abis_any_abi_feature_dict)
-                          {(SymbolRef ref_and_reloc_rec0, Some (''.text'', 1\<Colon>nat, 4\<Colon>nat)), (SymbolDef def_rec0, Some (''.data'', 0\<Colon>nat, 8\<Colon>nat))} None"])
-  apply(simp only: option.case foldl.simps annotated_memory_image.simps)+
-  apply(simp only: execute_two_steps_def load_image_def)
-  apply(simp only: x64_fetch_lemma1)
-  apply(simp only: Let_def split x64_decode_lemma Zinst.case)
-  apply(simp only: Run.simps instruction.case dfn'Zmov.simps read_cond.simps Zcond.case Let_def split)
-  apply(simp only: if_True ea_Zsrc.simps Zdest_src.case split fst_def EA.simps Zea.case)
-  apply(simp only: ea_Zdest.simps Zdest_src.case Zrm.case split fst_def ea_Zrm.simps ea_index.simps)
-  apply(simp only: option.case split ea_base.simps Zbase.case restrictSize.simps Zsize.case)
-  apply(simp only: write'EA.simps Zea.case split Zsize.case write'mem64.simps write'mem32.simps write'mem16.simps)
-  apply(simp only: write'mem8.simps snd_def split unit.case X64_state.simps add_0)
-  apply(simp only: load_program_def x64_fetch.simps Let_def split)
+  apply(rule impI)
+  apply safe
+  apply(frule possible_addresses_elim)
+  apply(drule encode_fixed_program_compute)
+  apply(simp only: Let_def)
+  apply clarify
+  apply(simp only: concat.simps append.simps)
+  apply(thin_tac "encode (Zmov (Z_ALWAYS, Z64, Zrm_i (Zm (None, ZnoBase, of_nat addr), 5\<Colon>64 word))) =
+       [72\<Colon>8 word, 199\<Colon>8 word, 4\<Colon>8 word, 37\<Colon>8 word, of_nat ((20\<Colon>nat) + (addr - (4194324\<Colon>nat))), 0\<Colon>8 word, 64\<Colon>8 word, 0\<Colon>8 word, 5\<Colon>8 word, 0\<Colon>8 word, 0\<Colon>8 word, 0\<Colon>8 word]")
+  apply(thin_tac "encode (Zmov (Z_ALWAYS, Z64, Zr_rm (RAX, Zm (None, ZnoBase, of_nat addr)))) =
+       [72\<Colon>8 word, 139\<Colon>8 word, 4\<Colon>8 word, 37\<Colon>8 word, of_nat ((20\<Colon>nat) + (addr - (4194324\<Colon>nat))), 0\<Colon>8 word, 64\<Colon>8 word, 0\<Colon>8 word]")
+  apply(simp only: load_fixed_program_instructions_def)
+thm build_fixed_program_memory_def
+  apply(simp add: build_fixed_program_memory_def)
 
-thm restrictSize.simps
-term MEM
-*)
 end
